thy/BDDCode.thy
@@ -1,3 +1,4 @@
+
 theory BDDCode
 imports LevelCollapse
 begin
